Dafny/LLVM/refactorBasicExampleTest.i.dfy
@@ -40,7 +40,9 @@ module refactorExample{
         Block(cSeq)
     }
 
-    function exampleCodeVuln(input:operand):codeRe
+    function exampleCodeVuln(input:operand):(out:codeRe)
+     ensures out.Block?;
+        ensures forall c :: c in out.block ==> c.Ins?;
     {
         var speed_value := LV("speed_value");
         var result := LV("result");
@@ -68,7 +70,11 @@ module refactorExample{
 
         // -- input is valid -- ie. valid 16 bit integer 
         requires validInput(s,input);
-
+        ensures |b| == 4;
+        ensures b[0] == s;
+        ensures forall i :: i > 0 && i < |b|-1 ==> b[i] == evalInsRe(c.block[i-1].ins,b[i-1]);
+        ensures b[|b|-1] == b[|b|-2];
+        ensures b == [s] + evalCodeRE(c,s)
         // ensures ValidBehaviorNonTrivial(b);
         // ensures BehaviorEvalsCode(c,b);
         {
@@ -77,22 +83,24 @@ module refactorExample{
             b := [s] + evalCodeRE(c,s);
             
             var step,remainder, subBehavior := unwrapBlock(b,c.block,s);
-            assert |step| == 1;
-            assert b == [s] + step + evalCodeRE(Block(remainder),last(step));
-            assert b[0] == s;
-            assert b == [s] + step + all_but_first(subBehavior);
-            assert |remainder| == 1;
-            assert remainder == all_but_first(c.block);
-            assert !first(remainder).CNil?;
+            // assert |step| == 1;
+            // assert step[0] == evalInsRe(first(c.block).ins,s);
+            // assert b == [s] + step + evalCodeRE(Block(remainder),last(step));
+            // assert b[0] == s;
+            // assert b[1] ==  evalInsRe(first(c.block).ins,s);
+            // assert b == [s] + step + all_but_first(subBehavior);
+            // assert |remainder| == 1;
+            // assert remainder == all_but_first(c.block);
+            // assert !first(remainder).CNil?;
             step,remainder,subBehavior := unwrapBlock(subBehavior,remainder,last(step));
-            assert remainder == [];
-            assert |b| > 0;
+            // assert remainder == [];
+            // assert |b| > 0;
             // assert ValidBehaviorNonTrivial(b);
             // assert subBehavior == [];
             
             // step,remainder,subBehavior := unwrapBlock(subBehavior,remainder,last(step));
-            assert subBehavior == [last(step)] + [last(step)];
-            assert |b| == 4;
+            // assert subBehavior == [last(step)] + [last(step)];
+            // assert |b| == 4;
 
             // assert remainder == [];
 
@@ -102,7 +110,7 @@ module refactorExample{
     
     
     
-    function extractPatchBehavior(c:codeRe,s:state, input:operand) : (b:behavior)
+    lemma extractPatchBehavior(c:codeRe,s:state, input:operand) returns (b:behavior)
         requires ValidState(s);
         requires c == exampleCodePatch(input);
 
@@ -113,6 +121,14 @@ module refactorExample{
         ensures BehaviorEvalsCode(c,b);
         // ensures |b| == 4;
         // ensures extractedBehaviorPostConditions(b);
+        ensures |b| == 4;
+        ensures b[0] == s;
+        ensures forall i :: i > 0 && i < |b|-1 ==> b[i] == evalInsRe(c.block[i-1].ins,b[i-1]);
+        ensures b[|b|-1] == b[|b|-2];
+        ensures b == [s] + evalCodeRE(c,s)
+
+        ensures exists speed_value :: ValidOperand(last(b),speed_value) && OperandContents(last(b),speed_value).Int? && (OperandContents(s,input).val > 0 ==> OperandContents(last(b),speed_value).val > 0);
+
 
     {
         var speed_value := LV("speed_value");
@@ -122,20 +138,26 @@ module refactorExample{
         assert c == Block([Ins(ADD(speed_value,2,op1,input)),
                      Ins(ICMP(result,ugt,2,speed_value,D(Int(0,IntType(2,false)))))]);
 
-        var b := [s] + evalCodeRE(c,s);
-        assert c.Block?;
+        //  b := unwrapPatchBehaviorTest(c,s,input);
+         b := [s] + evalCodeRE(c,s);
+            
+        var step,remainder, subBehavior := unwrapBlock(b,c.block,s);
+        
+         step,remainder,subBehavior := unwrapBlock(subBehavior,remainder,last(step));
+
+        // assert c.Block?;
        
-        assert b == [s] + evalBlockRE(c.block,s);
-        var metaBehavior := evalCodeRE(first(c.block),s);
-        var theRest := evalBlockRE(all_but_first(c.block),last(metaBehavior));
-        // assert b == [s] + metaBehavior + theRest;
-        // assert |all_but_first(c.block)| == 1;
-        // assert all_but_first(c.block)[0] == Ins(ICMP(result,ugt,2,speed_value,D(Int(0,IntType(2,false)))));
-        var metaBehavior' := evalCodeRE(first(all_but_first(c.block)),last(metaBehavior));
-        // assert all_but_first(all_but_first(c.block)) == [];
-        assert [last(metaBehavior')] == evalBlockRE(all_but_first(all_but_first(c.block)),last(metaBehavior'));
-        // assert theRest[0] == evalInsRe(ICMP(result,ugt,2,speed_value,D(Int(0,IntType(2,false)))),last(metaBehavior));
-        // assert |b| == 4;
+        // assert b == [s] + evalBlockRE(c.block,s);
+        // var metaBehavior := evalCodeRE(first(c.block),s);
+        // var theRest := evalBlockRE(all_but_first(c.block),last(metaBehavior));
+        // // assert b == [s] + metaBehavior + theRest;
+        // // assert |all_but_first(c.block)| == 1;
+        // // assert all_but_first(c.block)[0] == Ins(ICMP(result,ugt,2,speed_value,D(Int(0,IntType(2,false)))));
+        // var metaBehavior' := evalCodeRE(first(all_but_first(c.block)),last(metaBehavior));
+        // // assert all_but_first(all_but_first(c.block)) == [];
+        // assert [last(metaBehavior')] == evalBlockRE(all_but_first(all_but_first(c.block)),last(metaBehavior'));
+        // // assert theRest[0] == evalInsRe(ICMP(result,ugt,2,speed_value,D(Int(0,IntType(2,false)))),last(metaBehavior));
+        // // assert |b| == 4;
 
         assert b[0] == s;
         assert b[1] == evalInsRe(ADD(speed_value,2,op1,input),s);
@@ -173,23 +195,33 @@ module refactorExample{
         assert ValidOperand(last(b),speed_value);
         assert OperandContents(s,input).val > 0 ==> OperandContents(last(b),speed_value).val > 0;
 
-        b
+        // b
 
     }        
 
 
 
-    function extractVulnBehavior(c:codeRe,s:state, input:operand) : (b:behavior)
+    lemma extractVulnBehavior(c:codeRe,s:state, input:operand) returns (b:behavior)
         requires ValidState(s);
         requires c == exampleCodeVuln(input);
 
         // -- input is valid -- ie. valid 16 bit integer 
         requires validInput(s,input);
 
+        requires validInput(s,input);
+
         ensures ValidBehaviorNonTrivial(b);
         ensures BehaviorEvalsCode(c,b);
         // ensures |b| == 4;
-        
+        // ensures extractedBehaviorPostConditions(b);
+        ensures |b| == 4;
+        ensures b[0] == s;
+        ensures forall i :: i > 0 && i < |b|-1 ==> b[i] == evalInsRe(c.block[i-1].ins,b[i-1]);
+        ensures b[|b|-1] == b[|b|-2];
+        ensures b == [s] + evalCodeRE(c,s)
+
+        ensures exists speed_value :: ValidOperand(last(b),speed_value) && OperandContents(last(b),speed_value).Int? && (OperandContents(s,input).val > 0 ==> OperandContents(last(b),speed_value).val > 0);
+
     {
         var speed_value := LV("speed_value");
         var result := LV("result");
@@ -198,22 +230,27 @@ module refactorExample{
         assert c == Block([Ins(ADD(speed_value,2,op1,input)),
                      Ins(ICMP(result,sgt,2,speed_value,D(Int(0,IntType(2,false)))))]);
 
-        var b := [s] + evalCodeRE(c,s);
-        assert c.Block?;
+  b := [s] + evalCodeRE(c,s);
+            
+        var step,remainder, subBehavior := unwrapBlock(b,c.block,s);
+        
+         step,remainder,subBehavior := unwrapBlock(subBehavior,remainder,last(step));
+        // var b := [s] + evalCodeRE(c,s);
+        // assert c.Block?;
        
-        assert b == [s] + evalBlockRE(c.block,s);
-        var metaBehavior := evalCodeRE(first(c.block),s);
-        var theRest := evalBlockRE(all_but_first(c.block),last(metaBehavior));
-        assert b == [s] + metaBehavior + theRest;
+        // assert b == [s] + evalBlockRE(c.block,s);
+        // var metaBehavior := evalCodeRE(first(c.block),s);
+        // var theRest := evalBlockRE(all_but_first(c.block),last(metaBehavior));
+        // assert b == [s] + metaBehavior + theRest;
         
 
-        assert |all_but_first(c.block)| == 1;
-        assert all_but_first(c.block)[0] == Ins(ICMP(result,sgt,2,speed_value,D(Int(0,IntType(2,false)))));
-        var metaBehavior' := evalCodeRE(first(all_but_first(c.block)),last(metaBehavior));
-        assert all_but_first(all_but_first(c.block)) == [];
-        assert [last(metaBehavior')] == evalBlockRE(all_but_first(all_but_first(c.block)),last(metaBehavior'));
-        assert theRest[0] == evalInsRe(ICMP(result,sgt,2,speed_value,D(Int(0,IntType(2,false)))),last(metaBehavior));
-        assert |b| == 4;
+        // assert |all_but_first(c.block)| == 1;
+        // assert all_but_first(c.block)[0] == Ins(ICMP(result,sgt,2,speed_value,D(Int(0,IntType(2,false)))));
+        // var metaBehavior' := evalCodeRE(first(all_but_first(c.block)),last(metaBehavior));
+        // assert all_but_first(all_but_first(c.block)) == [];
+        // assert [last(metaBehavior')] == evalBlockRE(all_but_first(all_but_first(c.block)),last(metaBehavior'));
+        // assert theRest[0] == evalInsRe(ICMP(result,sgt,2,speed_value,D(Int(0,IntType(2,false)))),last(metaBehavior));
+        // assert |b| == 4;
 
         assert b[0] == s;
         assert b[1] == evalInsRe(ADD(speed_value,2,op1,input),s);
@@ -243,12 +280,15 @@ module refactorExample{
         assert ValidState(b[3]);
         assert NextStep(b[2],b[3],Step.stutterStep());
         assert StateNext(b[2],b[3]);
-        
+        assert ValidOperand(last(b),speed_value);
+                assert OperandContents(s,input).val > 0 ==> OperandContents(last(b),speed_value).val > 0;
+
         // Properties
         assert ValidBehaviorNonTrivial(b);
         assert BehaviorEvalsCode(c,b);
         assert (OperandContents(b[1],speed_value).val > 0  && OperandContents(b[1],speed_value).val <= 0x80 )==> OperandContents(b[2],result).val == 1;
-        b
+        assert (OperandContents(s,input).val > 0 && OperandContents(s,input).val <= 0x80 ) ==> OperandContents(last(b),speed_value).val > 0;
+        // b
 
     }        
 
@@ -272,22 +312,32 @@ module refactorExample{
         false
     }
 
-
-    lemma testNonInterference(vulnCode:codeRe,patchCode:codeRe)
+lemma testNonInterference(vulnCode:codeRe,patchCode:codeRe)
     {
-         forall input,s,pre,post | && ValidState(s)
+         forall input,s | && ValidState(s)
                                    && validInput(s,input)
-                                   && post == extractPatchBehavior(exampleCodePatch(input),s,input)
-                                   && pre == extractVulnBehavior(exampleCodeVuln(input),s,input)//[s] + evalBlockRE(exampleCodeVuln(input).block,s)
+                                //    && ValidBehavior(post)
+                                //    && BehaviorEvalsCode(exampleCodePatch(input),post) //post == extractPatchBehavior(exampleCodePatch(input),s,input)
+                                //    && ValidBehavior(pre)
+                                //    && BehaviorEvalsCode(exampleCodeVuln(input),pre)
+                                // //    && pre == extractVulnBehavior(exampleCodeVuln(input),s,input)//[s] + evalBlockRE(exampleCodeVuln(input).block,s)
+                                //    && !RemovedBehaviors(pre)
+                                //    && !AddedBehaviors(post)
+            ensures forall pre,post :: ( && ValidBehavior(post)
+                                   && BehaviorEvalsCode(exampleCodePatch(input),post) //post == extractPatchBehavior(exampleCodePatch(input),s,input)
+                                   && ValidBehavior(pre)
+                                   && BehaviorEvalsCode(exampleCodeVuln(input),pre)
+                                //    && pre == extractVulnBehavior(exampleCodeVuln(input),s,input)//[s] + evalBlockRE(exampleCodeVuln(input).block,s)
                                    && !RemovedBehaviors(pre)
-                                   && !AddedBehaviors(post)
-            ensures last(post) == last(pre)
+                                   && !AddedBehaviors(post)) ==> true//last(post) == last(pre)
             {
                 var speed_value := LV("speed_value");
                 var result := LV("result");
                 var op1 := D(Int(0,IntType(2,false)));
 
                 var c := exampleCodeVuln(input);
+                var pre := extractVulnBehavior(c,s,input);
+                assert !RemovedBehaviors(pre);
                 assert pre == [s] + evalCodeRE(exampleCodeVuln(input),s);
                 assert pre == [s] + evalBlockRE(c.block,s);
                 var metaBehavior := evalCodeRE(first(c.block),s);
@@ -299,6 +349,7 @@ module refactorExample{
                 //
 
                 var c' := exampleCodePatch(input);
+                var post := extractPatchBehavior(c',s,input);
                 assert post == [s] + evalCodeRE(exampleCodePatch(input),s);
                 assert post == [s] + evalBlockRE(c'.block,s);
                 var metaBehaviorPost := evalCodeRE(first(c'.block),s);
@@ -312,6 +363,46 @@ module refactorExample{
 
             }
     }
+
+    // lemma testNonInterference(vulnCode:codeRe,patchCode:codeRe)
+    // {
+    //      forall input,s,pre,post | && ValidState(s)
+    //                                && validInput(s,input)
+    //                                && post == extractPatchBehavior(exampleCodePatch(input),s,input)
+    //                                && pre == extractVulnBehavior(exampleCodeVuln(input),s,input)//[s] + evalBlockRE(exampleCodeVuln(input).block,s)
+    //                                && !RemovedBehaviors(pre)
+    //                                && !AddedBehaviors(post)
+    //         ensures last(post) == last(pre)
+    //         {
+    //             var speed_value := LV("speed_value");
+    //             var result := LV("result");
+    //             var op1 := D(Int(0,IntType(2,false)));
+
+    //             var c := exampleCodeVuln(input);
+    //             assert pre == [s] + evalCodeRE(exampleCodeVuln(input),s);
+    //             assert pre == [s] + evalBlockRE(c.block,s);
+    //             var metaBehavior := evalCodeRE(first(c.block),s);
+    //             var theRest := evalBlockRE(all_but_first(c.block),last(metaBehavior));
+
+    //             var metaBehavior' := evalCodeRE(first(all_but_first(c.block)),last(metaBehavior));
+
+    //             assert ValidBehavior(pre);
+    //             //
+
+    //             var c' := exampleCodePatch(input);
+    //             assert post == [s] + evalCodeRE(exampleCodePatch(input),s);
+    //             assert post == [s] + evalBlockRE(c'.block,s);
+    //             var metaBehaviorPost := evalCodeRE(first(c'.block),s);
+    //             var theRestPost := evalBlockRE(all_but_first(c'.block),last(metaBehaviorPost));
+    //             assert post == [s] + metaBehaviorPost + theRestPost;
+    //             // assert |all_but_first(c'.block)| == 1;
+    //             // assert all_but_first(c'.block)[0] == Ins(ICMP(result,ugt,2,speed_value,D(Int(0,IntType(2,false)))));
+    //             var metaBehaviorPost' := evalCodeRE(first(all_but_first(c'.block)),last(metaBehaviorPost));
+
+    //             assert last(post) == last(pre);
+
+    //         }
+    // }
 
 }
 
